\documentclass[../../solutions]{subfiles}
\title{Template}
\author{}
\begin{document}
\maketitle

\setexercise{4}{1}{4}
\begin{exercise}
  Prove that the construction of the free $R$-module on a set
  described in Example 4.1.10(v) is functorial.
\end{exercise}

\begin{proof}
  We wish to show that $\func{F}{\Set}{\Mod{R}}$ with $F(X)=R[X]$ is
  functorial.  Given $\func{f}{X}{Y}$ in \Set, we need to define
  $\func{Ff}{R[X]}{R[Y]}$.  Suppose that $\sum_{x\in X} a_xx\in R[X]$
  (writing this to mean $(a_x)_{x\in R}$).  We define
  $$Ff\left(\sum_{x\in X} a_xx\right) = \sum_{x\in X} a_xf(x)$$
  which is a finite formal sum in $R[Y]$.  We first show that this is
  a morphism $R[X]\to R[Y]$ in \Mod{R}, and then we show this it is
  functorial.

  For any elements of $R[X]$ and any $r\in R$, we have:
  \begin{align*}
    Ff\left(\sum_{x\in X} a_xx+\sum_{x\in X} b_xx\right)
         &=Ff\left(\sum_{x\in X} (a_x+b_x)x\right) \\
         &=\sum_{x\in X} (a_x+b_x)f(x) \\
         &= \sum_{x\in X} a_xf(x)+\sum_{x\in X} b_xf(x) \\
         &= Ff\left(\sum_{x\in X} a_xx\right)+Ff\left(\sum_{x\in X}
           b_xx\right)
  \end{align*}
  and
  \begin{align*}
    Ff\left(r\sum_{x\in X} a_xx\right)
         &= Ff\left(\sum_{x\in X} ra_xx\right) \\
         &= \sum_{x\in X} ra_xf(x) \\
         &= r\sum_{x\in X} a_xf(x) \\
         &= rFf\left(\sum_{x\in X} a_xx\right)
  \end{align*}
  so $Ff$ is a morphism as required.

  For functoriality, we need to show that $F1_X=1_{FX}$, and if
  $\func{f}{X}{Y}$ and $\func{g}{Y}{Z}$, then $F(gf)=Fg\cdot Ff$.
  For the first, we have
  \begin{align*}
    F1_X\left(\sum_{x\in X} a_xx\right)
    &= \sum_{x\in X} a_x1_X(x) \\
    &= \sum_{x\in X} a_xx \\
    &= 1_{R[X]}\left(\sum_{x\in X} a_xx\right)
  \end{align*}
  so $F1_X=1_{FX}$.  For the second, we have
  \begin{align*}
    F(gf)\left(\sum_{x\in X} a_xx\right)
    &= \sum_{x\in X} a_xgf(x) \\
    &= Fg\left(\sum_{x\in X} a_xf(x)\right) \\
    &= Fg\left(Ff\left(\sum_{x\in X} a_xx\right)\right) \\
    &= (Fg\cdot Ff)\left(\sum_{x\in X} a_xx\right) \\
  \end{align*}
  so $F(gf)=Fg\cdot Ff$.

  Therefore the construction described is functorial.
\end{proof}

\end{document}
